liveness start

lemma/liveness.v
@@ -2,7 +2,7 @@
 From Paco Require Import paco pacotac.
 From SST Require Import src.expr src.header src.local CpdtTactics src.lcontext.
 From SST Require Import src.global src.projection src.part  src.balanced src.merge src.wfltt src.gttreeh.
-From SST Require Import lemma.projection lemma.projection_helper lemma.decidable lemma.soundness.
+From SST Require Import lemma.projection lemma.projection_helper lemma.decidable lemma.liveness_helpers lemma.soundness.
 From SST Require Import src.step lemma.step src.assoc lemma.completeness src.ltth src.path_props.
 Require Import List String Coq.Arith.PeanoNat Morphisms Relations Setoid.
 Require Import Coq.Program.Equality.
@@ -12,1747 +12,504 @@ From Equations Require Import Equations.
 
 Import ListNotations.
 
-Definition gttstepRel g g' := exists p q ell, gttstepC g g' p q ell.
-
-Definition gttstepRtc := clos_refl_trans gtt gttstepRel.
-
-Locate tctxRtc.
-
-Lemma tctxR_invariance (P:tctx -> Prop): forall gamma gamma', 
-    P gamma -> (forall a b , P a -> tctxRcomm a b -> P b) ->
-    tctxRtc gamma gamma'-> P gamma'.
-Proof.
-    intros;induction H1;crush.
-Qed.
-
-Lemma tctx_wf_after_rtc : forall gamma gamma', 
-tctx_wf gamma -> tctxRtc gamma gamma' -> tctx_wf gamma'.
-Proof.
-    intros.
-    pattern gamma'. 
-    eapply tctxR_invariance with (gamma:=gamma);try easy.
-    intros. red in H2;destr_hyps;subst. Search tctx_wf tctxR.
-    eapply tctx_wf_after_red_comm;[| exact H2];easy.
-Qed.
-
-Lemma tctxR_invariance_wf (P:tctx -> Prop): forall gamma gamma', 
-    tctx_wf gamma ->
-    P gamma -> (forall a b , tctx_wf a -> P a -> tctxRcomm a b -> P b) ->
-    tctxRtc gamma gamma'-> P gamma'.
-Proof.
-    intros.  induction H2;crush.
-    eapply IHclos_refl_trans2;try easy.
-    fold tctxRtc in H2_.
-    eapply tctx_wf_after_rtc with (gamma:=x);try easy.
-Qed.
-
-Lemma assoc_preservation_context: forall gamma gamma' g, tctx_wf gamma -> 
-tctxRtc gamma gamma' ->
-    wfgC g ->
-    assoc gamma g -> exists g', assoc gamma' g' /\ wfgC g'.
-Proof.
-    intros.
-    pattern gamma'.
-    set (P:=(fun t : tctx => exists g' : gtt, assoc t g' /\ wfgC g')).
-
-    specialize (tctxR_invariance_wf P) as Hinv.
-    eapply Hinv with (gamma:=gamma);try easy. red. exists g;easy.
-    
-    intros. unfold P in *. red in H5;destr_hyps. 
-    eapply assoc_completeness in H5;try easy.
-    destr_hyps. exists x3. split;try easy.
-    
-    eapply wfgC_after_step in H7;try easy.
-    eapply assoc_implies_projectable;easy.
-Qed.
-
-Check typ_p_gtth.
-Check ishParts.
-
-Inductive is_tree_prefix : gtth -> gtth -> Prop :=
-    | tree_prefix_hole : forall n g, is_tree_prefix (gtth_hol n) g
-    | tree_prefix_tree : forall p q xs ys,
-    Forall2 (fun u v => (u=None /\ v=None)
-                \/ exists s g1 g2, u=Some (s, g1) /\ v=Some (s,g2) /\
-                is_tree_prefix g1 g2
-            ) xs ys ->
-    is_tree_prefix (gtth_send p q xs) (gtth_send p q ys).
-  
-
-Section tree_prefix_ind_ref.
-  Variable P : gtth -> gtth -> Prop.
-  Hypothesis P_hol : forall n g, P  (gtth_hol n ) g.
-  Hypothesis P_send : forall p q xs ys, List.Forall2 (fun u v => (u = None /\ v = None) \/ 
-                                                 (exists s g g', u = Some(s, g) /\ v = Some(s, g') /\ P g g')) xs ys -> 
-                                                 P (gtth_send p q xs) (gtth_send p q ys).
-  
-  Fixpoint tree_prefix_ind_ref G G' (a : is_tree_prefix G G') {struct a} : P  G G'.
-  Proof.
-    destruct a.
-    {
-        apply P_hol.   
-    }
-    apply P_send.
-    eapply Forall2_mono in H as Hm. exact Hm.
-    intros.
-    simpl.
-    destruct H0;[crush|].
-    destr_hyps;subst.
-    right. exists x0, x1, x2.
-    crush.
-  Qed.
-End tree_prefix_ind_ref.
+Inductive gtth_eq: gtth -> gtth -> Prop :=
+    | gtth_eq_hol : forall n m, gtth_eq (gtth_hol n) (gtth_hol m)
+    | gtth_eq_send : forall xs ys p q , 
+    Forall2 (fun u v => (u=None /\ v=None) \/ (exists s g1 g2, u=Some (s,g1) /\ v=Some (s,g2) /\ gtth_eq g1 g2)) 
+    xs ys ->
+    gtth_eq (gtth_send p q xs) (gtth_send p q ys).
 
 
-Lemma prefix_height_helper: forall p q s t xs ys, 
-(*wfgtth (gtth_send p q xs) -> wfgtth (gtth_send s t ys) ->*)
-Forall2 (fun u v => (u=None /\ v=None) \/ exists s g g', u=Some (s,g) /\ v=Some (s,g') /\ gtth_height g <= gtth_height g') xs ys ->
-gtth_height (gtth_send p q xs) <= gtth_height (gtth_send s t ys).
-Proof.
-    intros.
-    generalize dependent ys.
-    generalize dependent xs.
-    induction xs.
-    {
-        intros. crush.   
-    }
-    {
-        intros.
-        destruct ys. inversion H.
-
-        inversion H;subst.
-        destruct a.
-        {
-            destruct H3;try easy.
-            destr_hyps;subst.
-            inversion H0;subst.
-            simpl.
-            eapply Arith_base.add_le_mono_r_proj_l2r.
-            eapply Nat.max_le_compat. easy.
-            assert (gtth_height (gtth_send p q xs) <= gtth_height (gtth_send s t ys)).
-            {
-                eapply IHxs;try easy.   
-            }
-            crush.
-        }
-        {
-            destruct H3;destr_hyps;try easy;subst. simpl.   
-            assert (gtth_height (gtth_send p q xs) <= gtth_height (gtth_send s t ys)).
-            {
-                eapply IHxs;try easy.   
-            }
-            crush.
-        }
-    }
-Qed.
-
-Lemma prefix_height_le : forall gc gp, wfgtth gc -> wfgtth gp -> is_tree_prefix gc gp -> gtth_height gc <= gtth_height gp.
-Proof.
-    intros * Hwfg1 Hwfg2 Hpref.
-    induction  Hpref using tree_prefix_ind_ref.
-    {
-        simpl;intros;
-        apply gtth_height_ge_0;easy.      
-    }
-    {
-        Search Forall2.
-        eapply prefix_height_helper.
-        eapply Forall2_forall.
-        eapply Forall2_length. exact H.
-        intros.
-        destruct (onth k xs) eqn:Hyg.
-        {
-            right.
-            eapply Forall2_prop_r in H; [ | exact Hyg].
-            destr_hyps.
-            destruct H0;try easy.
-            destr_hyps;subst. inversion H0;subst. exists x0, x1, x2.
-            crush.
-            inversion Hwfg1;subst. eapply Forall_prop in H6; [| exact Hyg].
-            destruct H6;try easy.
-            destr_hyps.
-            inversion H;subst.
-            inversion Hwfg2;subst; eapply Forall_prop in H9; [ | exact H1].
-            destruct H9;try easy;destr_hyps. inversion H5;subst. apply H2;easy.
-        }
-        {
-            left.
-            destruct (onth k ys) eqn:Hyg1;crush.
-            eapply Forall2_prop_l in H;[| exact Hyg1]. destr_hyps. destruct H0;try easy.
-            destr_hyps. crush.
-        } 
-    }
-Qed.
-
-Inductive is_tree_proper_prefix : gtth -> gtth -> Prop :=
-    | tree_proper_prefix_hole : forall n p q xs, is_tree_proper_prefix (gtth_hol n) (gtth_send p q xs)
-    | tree_proper_prefix_tree : forall p q xs ys,
-    Forall2 (fun u v => (u=None /\ v=None)
-                \/ exists s g1 g2, u=Some (s, g1) /\ v=Some (s,g2) /\
-                is_tree_proper_prefix g1 g2
-            ) xs ys ->
-    is_tree_proper_prefix (gtth_send p q xs) (gtth_send p q ys).
-
-
-Section tree_proper_prefix_ind_ref.
-  Variable P : gtth -> gtth -> Prop.
-  Hypothesis P_hol : forall n p q xs, P (gtth_hol n ) (gtth_send p q xs).
-  Hypothesis P_send : forall p q xs ys, List.Forall2 (fun u v => (u = None /\ v = None) \/ 
-                                                 (exists s g g', u = Some(s, g) /\ v = Some(s, g') /\ P g g')) xs ys -> 
-                                                 P (gtth_send p q xs) (gtth_send p q ys).
-  
-  Fixpoint tree_proper_prefix_ind_ref G G' (a : is_tree_proper_prefix G G') {struct a} : P  G G'.
-  Proof.
-    destruct a.
-    {
-        apply P_hol.   
-    }
-    apply P_send.
-    eapply Forall2_mono in H as Hm. exact Hm.
-    intros.
-    simpl.
-    destruct H0;[crush|].
-    destr_hyps;subst.
-    right. exists x0, x1, x2.
-    crush.
-  Qed.
-End tree_proper_prefix_ind_ref.
-
-Print projection.
-
-
-
-
-Lemma empty_not_wfgtth: forall p q, wfgtth (gtth_send p q []) -> False.
-Proof. intros. inversion H. crush. Qed.
-Lemma max_lt_compat: forall n m p q, n < m -> p< q -> Nat.max n p  < Nat.max m q.
-Proof. crush. Qed.
-
-Lemma gtth_height_unfold_once_some : forall p q xs a b, gtth_height (gtth_send p q (Some (a,b)::xs)) =
-Init.Nat.max (gtth_height b +1) (gtth_height (gtth_send p q xs)).
-Proof.
-    intros.
-    crush.
-Qed.
-
-Lemma gtth_height_unfold_once_none : forall p q xs, gtth_height (gtth_send p q (None::xs)) =
-Init.Nat.max (0) (gtth_height (gtth_send p q xs)).
-Proof.
-    intros.
-    crush.
-Qed.
-
-Lemma SList_by_Forall2 {A:Type}: forall (xs ys: list (option A)), Forall2 (fun u v => u=None /\ v=None \/ exists x1 x2, u=Some x1 /\ v=Some x2) xs ys->
-SList xs -> SList ys.
-Proof.
-    intros. destruct xs. inversion H0.
-    generalize dependent ys. 
-    generalize dependent o. induction xs.
-    {
-        intros;
-        inversion H;subst; destruct o; destruct H3;try easy;
-        destr_hyps; inversion H1;subst;
-        inversion H5;subst;easy.        
-    }
-    {
-        intros.
-        destruct ys;
-        inversion H;subst.
-        
-        destruct o;destruct H4;destr_hyps;subst;try easy;
-        (assert (Hnys: SList ys) by (eapply IHxs with (o:=a);try easy));
-        [inversion H1;subst;simpl;destruct ys|];try easy.
-    }
-Qed.
-Lemma proper_prefix_height_helper: forall p q s t xs ys, 
-wfgtth (gtth_send p q xs) -> wfgtth (gtth_send s t ys) ->
-Forall2 (fun u v => (u=None /\ v=None) \/ exists s g g', u=Some (s,g) /\ v=Some (s,g') /\ gtth_height g < gtth_height g') xs ys ->
-gtth_height (gtth_send p q xs) < gtth_height (gtth_send s t ys).
-Proof.
-    intros * Hwfg1 Hwfg2.
-    (*
-    destruct xs;destruct ys; try (apply empty_not_wfgtth in H);try (apply empty_not_wfgtth in H1);try easy.
-    *)
-    generalize dependent ys.
-    generalize dependent xs.
-    destruct xs.
-    intros. inversion Hwfg1;subst;inversion H2.
-    revert o.
-    induction xs.
-    {
-        intros.
-        destruct o.
-        {
-            inversion H;subst.
-            destruct H2;try easy. destr_hyps.
-            inversion H0;subst.
-            destruct l';[|inversion H4];crush.
-        }
-        inversion Hwfg1. inversion H2.   
-    }
-    {
-        intros.
-        destruct ys. inversion H.
-
-        inversion H;subst.
-        destruct o.
-        {
-            destruct H3;try easy. destr_hyps. inversion H0;subst.
-            do 2 rewrite gtth_height_unfold_once_some.
-            eapply max_lt_compat. crush.
-            eapply IHxs;try easy.
-            assert(SList (a::xs)) by (inversion Hwfg1;subst;try easy).
-            constructor;[| inversion Hwfg1;subst;inversion H8];easy.
-            assert (SList ys).
-            {
-                inversion Hwfg2;subst;simpl in H4.
-                destruct ys;try easy.   
-            }
-            constructor;inversion Hwfg2;inversion H8;try easy.
-        }
-        {
-            destruct H3;destr_hyps;try easy;subst.    
-            do 2 rewrite gtth_height_unfold_once_none.
-            do 2 rewrite (Nat.max_0_l).
-            eapply IHxs;try easy.
-            assert(SList (a::xs)) by (inversion Hwfg1;subst;try easy).
-            constructor;[| inversion Hwfg1;subst;inversion H7];easy.
-            assert (SList ys).
-            {
-                inversion Hwfg2;subst. simpl in H3.
-                destruct ys;try easy.   
-            }
-            constructor;inversion Hwfg2;inversion H7;try easy.
-        }
-    }
-Qed.
-
-Lemma gtth_height_gt_0 : forall p q xs, wfgtth ((gtth_send p q xs)) -> gtth_height (gtth_send p q xs) > 0.
-Proof.
-    intros;
-    destruct (gtth_height (gtth_send p q xs)) eqn:Hyg;
-    [
-        apply gtth_height_0_means_hol in Hyg|];crush.
-Qed.
-
-Lemma proper_prefix_height_le : forall gc gp, wfgtth gc -> wfgtth gp -> 
-    is_tree_proper_prefix gc gp -> 
-    gtth_height gc < gtth_height gp.
-Proof.
-    destruct gc;destruct gp;try easy;intros.
-    simpl gtth_height at 1.
-    specialize (gtth_height_gt_0 n0 n1 l) as Hgt.
-    apply Hgt in H0. crush.
-
-    rename l into xs, l0 into ys.
-    induction H1 using tree_proper_prefix_ind_ref.
-    {
-        simpl gtth_height at 1.  specialize (gtth_height_gt_0 p q xs0) as Hgt. crush.    
-    }
-    {
-        eapply proper_prefix_height_helper;try easy.
-        eapply Forall2_forall;
-        [eapply Forall2_length; exact H1|].
-        intros.
-        destruct (onth k xs0) eqn:Hyg.
-        {
-            right.
-            eapply Forall2_prop_r in H1;[ | exact Hyg].
-            destr_hyps.
-            destruct H2;try easy.
-            destr_hyps;subst. inversion H2;subst. exists x0, x1, x2.
-            crush.
-            inversion H;subst. eapply Forall_prop in H8; [| exact Hyg].
-            destruct H8;try easy.
-            destr_hyps.
-            inversion H1;subst.
-            inversion H0;subst; eapply Forall_prop in H11; [ | exact H3].
-            destruct H11;try easy;destr_hyps. inversion H7;subst. apply H4;easy.
-        }
-        {
-            left.
-            destruct (onth k ys0) eqn:Hyg1;crush.
-            eapply Forall2_prop_l in H1;[| exact Hyg1]. destr_hyps. destruct H2;try easy.
-            destr_hyps. crush.
-        }    
-    }
-Qed.
-
-Definition path_starts_with (gamma:tctx) (pt:Path):=
-  match pt with 
-  | cocons (a,b) _ => a=gamma
-  | _ => False
-  end.
-
-
-Lemma assoc_implies_part: forall p Tp gamma g, tctx_wf gamma  -> wfgC g -> assoc gamma g ->
-M.find p gamma = Some Tp -> Tp <> ltt_end -> isgPartsC p g.
-Proof.
-    intros.
-    destruct (decidable_isgPartsC g p);try easy.
-    tac_use_assoc H1 p H4.
-    specialize (Hassoc_u _ H2). easy. 
-Qed.
-
-Check balanced_to_tree.
-Print typ_p_gtth.
-
-Print projection.
-(*
-
-Inductive used_in_gtth : nat -> gtth -> Prop := 
-    | used_hol_gtth : forall n, used_in_gtth n (gtth_hol n)
-    | used_send_gtth : forall n xs p q k s ll, onth k xs = Some (s, ll) -> used_in_gtth n ll -> 
-    used_in_gtth n (gtth_send p q xs).
-
-Definition fills_holes_gtth (ls :list (option gtt)) (l : gtth) :=
-    forall n, used_in_gtth n l -> exists s, onth n ls = Some s.
-
-
-Definition Forall_used ctx (P:nat -> Prop) := forall n , used_in_gtth n ctx -> 
-    P n.
-
-Inductive projectionH : list (option gtt) -> gtth -> part -> ltt -> Prop :=
-    | projectionH_hol : forall gs p t n, 
-    fills_holes_gtth gs (gtth_hol n) ->
-    Forall_used  (gtth_hol n) (fun u=> exists g, onth u gs =Some g /\ projectionC g p t)->
-    projectionH gs (gtth_hol n) p t
-    | projectionH_send : forall gs  r p q t ghs ys,
-    fills_holes_gtth gs (gtth_send p q ghs) ->
-    (ishParts r (gtth_send p q ghs) -> False) ->
-    Forall2 (fun u v => u=None /\ v=None 
-    \/ exists s g t', u=Some (s,g) /\ v=Some t' /\ projectionH gs g r t') ghs ys  ->
-    isMerge t ys -> projectionH gs (gtth_send p q ghs) r t.
-
-Lemma fills_holes_cont: forall gs p q k xs s g', fills_holes_gtth gs (gtth_send p q xs) -> onth k xs = Some (s,g') ->
-fills_holes_gtth gs g'.
-Proof.
-    intros.
-    red in H. red. intros.
-    assert(used_in_gtth n (gtth_send p q xs)).
-    {
-        econstructor;[exact H0 | exact H1].   
-    }
-    specialize (H n H2). exact H.
-Qed.
-
-Lemma projectionH_corr_projectionC : forall gs ctx p Tp g, 
-wfgC g -> fills_holes_gtth gs ctx -> typ_p_gtth gs ctx p g ->
- projectionH gs ctx p Tp -> projectionC g p Tp.
-Proof. 
-    intros * Hwfg  Hfills Htyp_p Hprojh.
-    red in Htyp_p.
-    induction ctx using gtth_ind_ref.
-    {
-        destr_hyps.
-        destruct g.
-        {
-            constructor;try easy.
-            eapply Forall_forall. intros.
-            destruct x. right. exists g.
-            eapply in_some_implies_onth in H2. destr_hyps.
-            eapply Forall_prop in H1;[| exact H2]. destruct H1;try easy. destr_hyps.   
-        }   
-    }
-*)
-Search isMergeCtx Forall.
-Print isMergeCtx.
-
-Definition triple_opt_sum:= (fun u v w : option gtt =>
-u = None /\ v = None /\ w = None \/
-(exists t0 : gtt, u = None /\ v = Some t0 /\ w = Some
-t0) \/
-(exists t0 : gtt, u = Some t0 /\ v = None /\ w = Some
-t0) \/
-(exists t0 : gtt, u = Some t0 /\ v = Some t0 /\
-w = Some t0)).
-
-Lemma Forall3S_samesize {A:Type}: forall P (xs ys zs:list A), Forall3S P xs ys zs -> 
-Datatypes.length xs= Datatypes.length zs \/ Datatypes.length ys = Datatypes.length zs.
-Proof.
-    intros;induction H;crush.
-Qed.
-
-Lemma Forall2R_to_Forall2 {A:Type}: 
-forall (xs ys:list A) P,
-Forall2R P xs ys -> Datatypes.length xs = Datatypes.length ys ->
-Forall2 P xs ys.
-Proof.
-    intros.
-    induction H.
-    {
-        destruct ys;crush.   
-    }
-    {
-        constructor;try easy.
-        eapply IHForall2R.
-        simpl in H0. crush.   
-    }
-Qed.
-Search Forall2R Datatypes.length.
-Search Forall3S.
-
-Lemma triple_sum_trilemma: forall xs ys zs x n, Forall3S triple_opt_sum xs ys zs ->
-onth n zs = Some x -> onth n xs = Some x \/ onth n ys= Some x.
-Proof.
-    intros.
-    generalize dependent ys.
-    generalize dependent xs.
-    generalize dependent n.
-    induction zs.
-    {
-        intros.
-        rewrite onth_nil in H0. easy.
-    }
-    {
-        intros.
-        destruct xs;destruct ys;intros;inversion H;[crush | crush |];subst.
-        destruct n.
-        {
-            simpl in H0;subst.
-            red in H5.
-            destruct H5;crush.
-        }
-        {
-            simpl in H0.
-            simpl.
-            eapply IHzs;try easy.
-        }   
-    }
-Qed.
-
-
-Lemma Forall_merge_gs P: forall gs gss,
-P None -> isMergeCtx gs gss -> Forall (fun u=> u=None \/ exists g, u=Some g /\ Forall P g) gss ->
-Forall P gs.
-Proof.
-    intros * Hpn.
-    intros.
-    induction H.
-    {
-        intros.
-        eapply Forall_prop with (l:=0) in H0.
-        destruct H0;try easy. destr_hyps.
-        inversion H;subst.
-        2:simpl;reflexivity. easy. 
-    }
-    {
-        eapply IHisMergeCtx. inversion H0;try easy.   
-    }
-    {
-        eapply Forall_forall.
-        intros.
-        destruct x;try easy.
-        {
-            Search Forall3S.
-            Search isMergeCtx Forall.
-            eapply in_some_implies_onth in H2 as Hsome. destr_hyps. rename x into n.
-            eapply triple_sum_trilemma in H;[|exact H3].
-            inversion H0;subst.
-            destruct H.
-            {
-                specialize (IHisMergeCtx H7).
-                eapply Forall_prop in H;[|exact IHisMergeCtx];easy.
-            }
-            {
-                destruct H6;try easy;destr_hyps;subst.
-                inversion H4;subst.
-                eapply Forall_prop in H5;[|exact H];easy.
-            }
-        }
-    }
-Qed.
-
-Lemma triple_sum_or_prop_l :  forall xs ys zs x n, Forall3S triple_opt_sum xs ys zs ->
-onth n xs = Some x -> onth n zs = Some x.
-Proof.
-    intros * Hsum Honth.
-    unfold triple_opt_sum in Hsum.
-    Print Forall3S.
-    generalize dependent xs.
-    generalize dependent ys.
-    revert n.
-    induction zs.
-    {
-        intros.
-        inversion Hsum;subst; rewrite onth_nil in Honth;easy.   
-    }
-    {
-        intros.
-        destruct xs;destruct ys;intros; inversion Hsum;[crush | crush |];subst.
-        rewrite onth_nil in Honth;easy.
-        destruct n.
-        {
-            simpl.
-            simpl in Honth;subst.
-            destruct H3;crush.   
-        }
-        {
-            simpl in Honth.
-            simpl.
-            eapply IHzs;[exact H7|exact Honth].   
-        }
-    }
-Qed.
-
-Lemma triple_sum_or_prop_r :  forall xs ys zs x n, Forall3S triple_opt_sum xs ys zs ->
-onth n ys = Some x -> onth n zs = Some x.
-Proof.
-    intros * Hsum Honth.
-    unfold triple_opt_sum in Hsum.
-    Print Forall3S.
-    generalize dependent xs.
-    generalize dependent ys.
-    revert n.
-    induction zs.
-    {
-        intros.
-        inversion Hsum;subst; rewrite onth_nil in Honth;easy.   
-    }
-    {
-        intros.
-        destruct xs;destruct ys;intros; inversion Hsum;[crush | crush |];subst.
-        rewrite onth_nil in Honth;easy.
-        destruct n.
-        {
-            simpl.
-            simpl in Honth;subst.
-            destruct H3;crush.   
-        }
-        {
-            simpl in Honth.
-            simpl.
-            eapply IHzs;[exact Honth|exact H7].   
-        }
-    }
-Qed.
-
-Lemma Forall2R_length {A:Type} {B:Type}: forall (P:A -> B-> Prop) xs ys, Forall2R P xs ys -> Datatypes.length xs <= Datatypes.length ys.
-Proof.
-    intros;
-    induction H;crush.
-Qed.
-Lemma Forall2R_subset_trans {A:Type}: forall (xs ys zs: list (option A)),
-Forall2R (fun u v=> u=None \/ u=v) xs ys ->
-Forall2R (fun u v=> u=None \/ u=v) ys zs ->
-Forall2R (fun u v=> u=None \/ u=v) xs zs.
-Proof.
-    intros.
-    eapply Forall2_Forall.
-    {
-        eapply Forall2R_length in H, H0. crush.
-    }
-    {
-        intros.
-        destruct (onth k xs) eqn:Hyg.
-        {
-            eapply Forall2R_prop in H;[|exact Hyg].
-            destr_hyps;subst.
-            destruct H2;try easy.   
-            symmetry in H.
-            eapply Forall2R_prop in H0;[|exact H]. 
-            destr_hyps.
-            destruct H2;try easy;subst. right;easy.
-        }
-        left;easy.
-    }
-Qed.
-
-Lemma mergeCtx_onth_subset: 
-forall gs gs' gss n,
-isMergeCtx gs gss ->
-onth n gss = Some gs' ->
-Forall2R (fun u v : option gtt => u = None \/ u = v) gs' gs.
-Proof.
-    intros * Hmerge Honth.
-    generalize dependent n.
-    induction Hmerge.
-    {
-        intros.
-        destruct n. simpl in Honth. inversion Honth;subst.
-        Search Forall2R.
-        eapply Forall2_Forall;crush.
-        
-        simpl in Honth. rewrite onth_nil in Honth;easy.
-    }
-    {
-        intros.
-        destruct n; simpl in Honth;try easy.
-        eapply IHHmerge;exact Honth.
-    }
-    {
-        intros.
-        destruct n.
-        {
-            simpl in Honth;inversion Honth;subst.
-            Search Forall3S.
-            eapply Forall3S_to_Forall2_r;exact H.   
-        }
-        {
-            simpl in Honth.
-            specialize (IHHmerge _ Honth).
-            eapply Forall3S_to_Forall2_l in H.
-            eapply Forall2R_subset_trans;[exact IHHmerge|];easy.
-        }
-    }
-Qed.
-
-Lemma Forall_subset {A:Type}: forall gs gs' (P: option A -> Prop), Forall2R (fun u v  => u = None \/ u = v) gs' gs -> P None -> 
-Forall P gs -> Forall P gs'.
-Proof.
-    intros.
-    eapply Forall_forall.
-    intros.
-    destruct x;try easy.
-    eapply in_some_implies_onth in H2 as Hsome.
-    destr_hyps.
-    eapply Forall2R_prop in H;[|exact H3].
-    destr_hyps.
-    destruct H4;crush.
-    symmetry in H4.
-    eapply Forall_prop in H1;[|exact H4].
-    crush.
-Qed.
-
-Lemma restricted_grafting_send : forall gs ctx p q g xs, 
-wfgC g -> projectableA g -> typ_gtth gs ctx g -> 
-(ishParts p ctx -> False) ->
-usedCtx gs ctx ->
-projectionC g p (ltt_send q xs) -> 
-Forall
-(fun u : option gtt =>
-u = None \/
-(exists (q : opt_lbl) (lsg : list (option (sort * gtt))),
-u = Some (gtt_send p q lsg) \/
-u = Some (gtt_send q p lsg) \/ u = Some gtt_end))
-gs -> 
-Forall (fun u=> u=None\/ exists ys, u=Some (gtt_send p q ys
-)) gs.
-Proof.
-    intros * Hwfg  Hprojable Hgraft Hishparts Hused Hprojp Hgraftcond.
-    
-    generalize dependent g.
-    generalize dependent gs.
-    generalize dependent ctx.
-    induction ctx using gtth_ind_ref.
-    {
-        intros.
-        destruct g;[pinversion Hprojp;apply proj_mon|].
-        eapply typ_gtth_hole_inv in Hgraft;try easy. destr_hyps;subst.
-        eapply extendLis_forall. split;[|left;easy].
-        
-        right. exists x. eapply Forall_prop in Hgraftcond;[|rewrite extendExtract;easy].
-        destruct Hgraftcond; try easy. destr_hyps.
-        destruct H;[|destruct H];inversion H;subst;pinversion Hprojp;crush;apply proj_mon.   
-    }
-    {
-        intros.
-        destruct g;[pinversion Hprojp;apply proj_mon|].
-        inversion Hgraft;subst.
-        rename n into s, n0 into t, xs0 into ghs, l into gcs.
-        inversion Hused;subst.
-        (*
-        eapply slist_implies_some in H3 as Hsome. destr_hyps;subst.
-        eapply Forall_prop in H;[|exact H0]. destruct H;try easy. destr_hyps.
-        
-        inversion H;subst. clear H.
-       *)
-       eapply Forall_merge_gs;[|exact H4 | ].
-        left. easy.
-
-        eapply Forall_forall.
-        intros.
-        destruct x;[|crush].
-        right. eapply in_some_implies_onth in H0 as Hsome.
-        destr_hyps.
-        exists l.
-        split;try easy.
-        eapply Forall2_prop_r in H6;[|exact H1].
-        destr_hyps.
-        destruct H5;try easy.
-        destr_hyps.
-        inversion H5;subst.
-        rename x1 into ctx1,x2 into s1, x3 into ghs1.
-        eapply Forall_prop in H as IH;[|exact H6].
-        destruct IH;try easy;destr_hyps;inversion H2;subst.
-        eapply Forall2_prop_r in H8 as Hgraftn;try exact H6.
-        destr_hyps. 
-        destruct H11;subst;try easy.
-        destr_hyps. inversion H10;subst.
-        rename x4 into g', x3 into ctx'.
-        eapply mergeCtx_onth_subset with (gs:=gs) in H1 as Hsubs;try easy.
-        assert (Hsp_noteq: s <> p).
-        {
-            red.
-            intros;subst. apply Hishparts.
-            apply ha_sendp.   
-        }
-        assert (Htp_noteq: t <> p).
-        {
-            red.
-            intros;subst. apply Hishparts.
-            apply ha_sendq.   
-        }
-        eapply H9 with (g:=g');try easy.
-        {
-            intros.
-            eapply Hishparts. econstructor;try exact H13;try easy;exact H6.
-        }
-        {
-            eapply Forall_subset with (gs:=gs);crush.   
-        }
-        {
-            eapply continuation_wfgC;[exact Hwfg|exact H11].   
-        }
-        {
-            Search projectableA gttstepC.
-            eapply projectable_after_step with (g:=(gtt_send s t gcs));try easy.
-            pfold.
-            econstructor.
-            2:symmetry in H11;exact H11.
-            Search wfgC (_ <> _).
-            eapply wfgC_triv in Hwfg as Hw. easy.
-        }
-        {
-            Search typ_gtth usedCtx.
-            eapply decidable_helper.typh_with_less;try exact Hsubs;easy.   
-        }
-        {
-            pinversion Hprojp;try apply proj_mon;crush.
-            eapply Forall2_prop_r in H22;[|exact H11].
-            destr_hyps.
-            destruct H14;try easy. destr_hyps;subst.
-            inversion H14;subst.
-            destruct H20;try easy.
-            Search isMerge onth.
-            eapply merge_inv_ss in H23;[|exact H15];subst.
-            easy.  
-        }  
-    }
-Qed. 
-
-Print projection.
-
-Lemma inequality_by_not_ishparts: forall p0 p q xs, (ishParts p0 (gtth_send p q xs) -> False) ->
-                            p0 <> p /\ p0 <> q.
-                            Proof.
-                                intros;split;red;intros;exfalso;apply H;subst;constructor.
-                            Qed.
-
-Inductive projectionH : gtth -> (list (option gtt)) -> part -> ltth ->
-(list (option ltt)) -> Prop :=
-    | projectionH_hol : forall n m r g t gs ls,
-    onth n gs= Some g -> onth m ls =Some t ->
-    projectionC g r t -> 
-    projectionH (gtth_hol n) gs r (ltth_hol m) ls
-    | projectionH_recv: forall p r gs ls xs ys, p <> r ->
-    Forall2
-    (fun (u : option (sort * gtth))
-    (v : option (sort * ltth)) =>
-    u = None /\ v = None \/
-    (exists (s : sort) (g : gtth) (t : ltth),
-    u = Some (s, g) /\ v = Some (s,t) /\ projectionH g gs r t ls))
-    xs ys -> projectionH (gtth_send p r xs) gs r (ltth_recv p ys) ls
-    | projectionH_send: forall p r gs ls xs ys, p <> r ->
-    Forall2
-    (fun (u : option (sort * gtth))
-    (v : option (sort * ltth)) =>
-    u = None /\ v = None \/
-    (exists (s : sort) (g : gtth) (t : ltth),
-    u = Some (s, g) /\ v = Some (s,t) /\ projectionH g gs r t ls))
-    xs ys -> projectionH (gtth_send r p xs) gs r (ltth_send p ys) ls
-    | projectionH_cont: forall p q r t twt k xs ys gs ls, p <> q ->
-        q <> r ->
-        p <> r ->
-        Forall2
-        (fun (u : option (sort * gtth)) (v : option ltth) =>
-        u = None /\ v = None \/
-        (exists (s : sort) (g : gtth) (t0 : ltth),
-        u = Some (s,g) /\ v=Some t0 /\ projectionH g gs r t0 ls)) xs
-        ys -> onth k  ys=Some t-> Forall (fun u=> u=None \/  exists th, u=Some th /\
-        typ_ltth th ls twt) ys ->
-         projectionH (gtth_send p q xs) gs
-        r t ls
-    .
-
-Ltac tac_forall_to_length := repeat (match goal with [H: Forall2 _ ?a ?b|- _] =>
-                apply Forall2_length in H |
-                [H: Forall2R _ ?a ?b|- _] =>
-                apply Forall2R_length in H
-                end);crush.
-
-Ltac tac_clear_id:= repeat match goal with [ H : ?a = ?a |- _ ] => clear H end.
-
-Ltac tac_use_forall2 Hforall2 Honth :=
-                    match Hforall2 with 
-                    (Forall2 _ ?a ?b) => match Honth with 
-                        (onth ?k ?a = Some ?p) => 
-                        eapply Forall2_prop_r in Hforall2;try exact Honth
-                        |
-                        (onth ?k ?b = Some ?p) => 
-                        eapply Forall2_prop_l in Hforall2;try exact Honth
-                        end     
-                    end. 
-                    Ltac tac_remove_dilemma :=
-                    match goal with 
-                    [ H: ?a \/ ?b |- _] => destruct H;try easy end.
-                    Ltac tac_inv_some := match goal with 
-                    [H: Some ?a = Some ?b |- _] => inversion H;subst end.
-                    Ltac tac_sanitize := destr_hyps;tac_remove_dilemma;destr_hyps;tac_inv_some;tac_clear_id.
-
-Lemma projectionH_consistent: forall gs gx ls lx p r g Tr, 
-wfgC g ->
+Lemma projectionH_ishparts: forall gs gx r p ls lx, 
 wfgtth gx ->
-typ_p_gtth gs gx p g ->
-projectionC g r Tr ->
-projectionH gx gs r lx ls -> typ_ltth lx ls Tr.
+(ishParts p gx -> False) -> projectionH gx gs r lx ls ->
+(ishlParts p lx ->False).
 Proof.
-    intros * Hwfg Hwfgth Htyp Hprojp Hprojhp.
-    generalize dependent gs.
-    generalize dependent g.
-    revert ls lx Tr.
-    generalize dependent gx.
+    intros *. revert gs r p ls lx. generalize dependent gx.
     induction gx using gtth_ind_ref.
     {
-        intros.
-        inversion Hprojhp;subst.
-        constructor.
-        red in Htyp. destr_hyps.
-        inversion H;subst.
-        rewrite H0 in H7. inversion H7;subst.
-        eapply proj_inj in Hprojp;try exact H2;subst;try easy.
+        intros. inversion H1;subst;inversion H2.
     }
     {
-        intros.
-        rename H into IH.
-        destruct (Nat.eq_dec p0 r);   
-        destruct (Nat.eq_dec q r);subst;try easy.
+        intros * Hwfg Hishparts Hproj Hishlparts.
+        inversion Hproj;subst.
         {
-            red in Htyp;destr_hyps. inversion H;subst. apply wfgC_triv in Hwfg;try easy.         
+            assert(Hslist: SList xs) by (inversion Hwfg;try easy).
+            inversion Hishlparts;subst;[exfalso;apply Hishparts;constructor |].
+            eapply Forall2_prop_l in H8;try exact H4;tac_sanitize.
+            eapply Forall_prop in H;try exact H1;tac_sanitize.
+            eapply H0 with (p:=p0);try exact H6;try easy.
+            subtac_wfgth_by_onth. subtac_ishparts_by_onth.
         }
         {
-            red in Htyp;destr_hyps.
-            inversion H;subst.
-            pinversion Hprojp;subst;try easy;try apply proj_mon.
-            {
-                exfalso. apply H2. apply decidable_helper.triv_pt_p;easy.   
-            }
-            inversion Hprojhp;subst;try easy.
-            {
-                eapply typ_ltth_send.
-                eapply Forall2_forall;[tac_forall_to_length;crush |].
-                rename xs into ghs, ys into gcs, ys0 into lcs, ys1 into lhs.
-                intros.
-                destruct (onth k lhs) eqn:Hyg.
-                {
-                    right.
-                    eapply Forall2_prop_l in H16;try exact Hyg.
-
-                    tac_sanitize.
-                    exists x0, x2. 
-                    eapply Forall2_prop_r in H8;try exact H3;tac_sanitize.
-                    eapply Forall2_prop_r in H11;try exact H6;tac_sanitize.
-                    eapply Forall_prop in IH;try exact H3;tac_sanitize.
-                    exists x6.
-                    (repeat split);try easy.
-                    eapply H4 with (gs:=gs) (g:=x1);try easy.
-                    {
-                        inversion Hwfgth;subst.
-                        eapply Forall_prop in H17;try exact H3. 
-                        tac_sanitize;easy. 
-                    }
-                    {
-                        eapply continuation_wfgC;try exact H6;try exact Hwfg.   
-                    }
-                    {
-                        destruct H12;try easy.   
-                    }
-                    {
-                        red.
-                        (repeat split);try easy.
-                        intros.
-                        eapply H0. eapply ha_sendr;try exact H3;try exact H16;try easy.
-                        1-2:red;intros;exfalso;subst;apply H0; constructor.   
-                    }         
-                }
-                {
-                    left;split;try easy.
-                    destruct (onth k lcs) eqn:Hyg1;try easy.
-                    eapply Forall2_prop_l in H11;try exact Hyg1;tac_sanitize.
-                    eapply Forall2_prop_l in H8;try exact H3;tac_sanitize.
-                    eapply Forall2_prop_r in H16;try exact H4;tac_sanitize.
-                    rewrite Hyg in H11;easy.
-                }
-            }   
+            
+            assert(Hslist: SList xs) by (inversion Hwfg;try easy).
+            inversion Hishlparts;subst;[exfalso;apply Hishparts;constructor |].
+            eapply Forall2_prop_l in H8;try exact H4;tac_sanitize.
+            eapply Forall_prop in H;try exact H1;tac_sanitize.
+            eapply H0 with (p:=p0);try exact H6;try easy.
+            subtac_wfgth_by_onth. subtac_ishparts_by_onth.
         }
         {
-            red in Htyp;destr_hyps.
-            inversion H;subst.
-            pinversion Hprojp;subst;try easy;try apply proj_mon.
-            {
-                exfalso. apply H2. apply decidable_helper.triv_pt_q;easy.   
-            }
-            inversion Hprojhp;subst;try easy.
-            {
-                eapply typ_ltth_recv.
-                eapply Forall2_forall;[tac_forall_to_length;crush |].
-                rename xs into ghs, ys into gcs, ys0 into lcs, ys1 into lhs.
-                intros.
-                destruct (onth k lhs) eqn:Hyg.
-                {
-                    right.
-                    eapply Forall2_prop_l in H16;try exact Hyg.
-
-                    tac_sanitize.
-                    exists x0, x2. 
-                    eapply Forall2_prop_r in H8;try exact H3;tac_sanitize.
-                    eapply Forall2_prop_r in H11;try exact H6;tac_sanitize.
-                    eapply Forall_prop in IH;try exact H3;tac_sanitize.
-                    exists x6.
-                    (repeat split);try easy.
-                    eapply H4 with (gs:=gs) (g:=x1);try easy.
-                    {
-                        inversion Hwfgth;subst.
-                        eapply Forall_prop in H17;try exact H3. 
-                        tac_sanitize;easy. 
-                    }
-                    {
-                        eapply continuation_wfgC;try exact H6;try exact Hwfg.   
-                    }
-                    {
-                        destruct H12;try easy.   
-                    }
-                    {
-                        red.
-                        (repeat split);try easy.
-                        intros.
-                        eapply H0. eapply ha_sendr;try exact H3;try exact H16;try easy.
-                        1-2:red;intros;exfalso;subst;apply H0; constructor.   
-                    }         
-                }
-                {
-                    left;split;try easy.
-                    destruct (onth k lcs) eqn:Hyg1;try easy.
-                    eapply Forall2_prop_l in H11;try exact Hyg1;tac_sanitize.
-                    eapply Forall2_prop_l in H8;try exact H3;tac_sanitize.
-                    eapply Forall2_prop_r in H16;try exact H4;tac_sanitize.
-                    rewrite Hyg in H11;easy.
-                }
-            }   
-        }
-        {
-            red in Htyp;destr_hyps.
-            inversion H;subst.
-            pinversion Hprojp;subst;try easy;try apply proj_mon.
-            {
-
-                inversion Hprojhp;subst;[
-                exfalso;apply H2; apply decidable_helper.triv_pt_q;easy
-                |exfalso;apply H2; apply decidable_helper.triv_pt_p;easy |]
-                .
-                eapply Forall_prop in H17;try exact H16.
-                tac_sanitize.
-                eapply Forall2_prop_l in H11;try exact H16.
-                tac_sanitize.
-                eapply Forall2_prop_r in H8;try exact H5;tac_sanitize.
-                eapply Forall_prop in IH;try exact H5.
-                tac_sanitize.
-                eapply H8 with (gs:=gs) (g:=x5);try easy.
-
-                inversion Hwfgth;subst; eapply Forall_prop in H18;try exact H5; tac_sanitize;easy.
-
-                eapply continuation_wfgC;try exact Hwfg;try exact H11.
-                pfold. 
-
-                constructor. intros;apply H2.
-                Search isgPartsC onth. eapply part_parent;try exact H11;try easy.
-                red. (repeat split);try easy.
-                intros.
-                eapply H0. 
-                eapply ha_sendr;try exact H5;try easy.
-                1-2:red;intros;exfalso;subst;apply H0; constructor.
-            }
-            {
-                inversion Hprojhp;subst;try easy.
-                eapply Forall_prop in H22;try exact H21;tac_sanitize.
-                eapply Forall2_prop_l in H16;try exact H21;tac_sanitize.
-                eapply Forall2_prop_r in H8;try exact H4;tac_sanitize.
-                eapply Forall_prop in IH;try exact H4;tac_sanitize.
-                eapply H8 with (g:=x5) (gs:=gs);try easy.   
-                {
-                 inversion Hwfgth;subst.
-                        eapply Forall_prop in H23;try exact H4. 
-                        tac_sanitize;easy.    
-                }
-                {
-                    eapply continuation_wfgC;try exact H16;try exact Hwfg.   
-                }
-                {
-                      eapply Forall2_prop_r in H13; try exact H16;tac_sanitize.
-                  
-                    eapply merge_inv_ss in H19;try exact H14;subst.
-                    destruct H20;try easy.
-                }
-                {
-                    red.
-                    (repeat split);try easy. intros.
-                    apply H0. econstructor;try exact H4;try easy.   
-                    1-2:red;intros;exfalso;subst;apply H0; constructor.   
-                }
-            }
-        }
-    }
-Qed.
-
-Print typ_p_recv_ltth.
-
-Lemma extendLis_length {A:Type}: forall (a b: option A) n, Datatypes.length (extendLis n a)=
-Datatypes.length (extendLis n b).
-Proof.
-    induction n;crush.
-Qed.
-
-Definition forall_projable gs :=Forall (fun u=>u=None \/ exists g, u=Some g /\ projectableA g) gs.
-Definition forall_wfg gs :=Forall (fun u=>u=None \/ exists g, u=Some g /\ wfgC g) gs.
-
-Lemma project_list: forall gs p q, Forall (fun u=> u=None\/ exists ys, u=Some (gtt_send p q ys)) gs ->
-forall_projable gs->
-forall_wfg gs ->
-exists ls, Forall2 (fun u v => u=None /\ v=None \/ exists g t, u=Some g /\ v=Some t /\ projectionC g q t) gs ls
-/\ Forall (fun u=> u=None \/ exists ys, u=Some (ltt_recv p ys)) ls.
-Proof.
-    intros * Hgs Hproj Hwfg.
-    induction gs.
-    {
-        exists []. split;constructor.   
-    }
-    {
-        inversion Hgs.
-        inversion Hproj.
-        inversion Hwfg.
-        destruct a;subst.
-        {
-            tac_sanitize.
-            specialize (IHgs H2 H6 H10);destr_hyps.
-            repeat tac_sanitize.
-            specialize (H5 q);destr_hyps.
-            pinversion H1;subst;try apply proj_mon;try easy;
-            [exfalso;apply H4;apply decidable_helper.triv_pt_q|];try easy.
-            exists (Some (ltt_recv p ys) :: x0).
-            split;constructor;try easy.
-            {
-                right. exists (gtt_send p q x) , (ltt_recv p ys);crush.
-                pfold;easy.   
-            }
-            {
-                right. exists ys. easy.   
-            }
-        }
-        {
-            specialize (IHgs H2 H6 H10);destr_hyps.
-            exists (None::x).
-            split;constructor;crush.   
+            eapply Forall2_prop_l in H6;try exact H11;tac_sanitize.
+            
+            eapply Forall_prop in H;try exact H1;tac_sanitize.
+            eapply H0 with (p:=p0);try exact H6;try easy.
+            subtac_wfgth_by_onth.
+            subtac_ishparts_by_onth.   
         }   
     }
 Qed.
 
-Definition gttstepC_any g g':= exists p q ell, gttstepC g g' p q ell. 
-Definition gttstepC_RT := clos_refl_trans gtt gttstepC_any.
+Lemma proj_contains_q_implies_part_send : forall g p q xs,
+wfgC g -> projectableA g ->
+projectionC g p (ltt_send q xs) ->
 
-Lemma extend_onth_inv {A:Type}: forall n (a:A) b n', onth n (extendLis n' (Some a))=Some b ->
-n=n'.
+isgPartsC p g/\ isgPartsC q g.
 Proof.
-    intros.
-    generalize dependent n.
-    induction n'.
-    {
-        simpl.
-        destruct n;crush.
-        rewrite onth_nil in H;easy.   
-    }
-    {
-        destruct n.
-        {
-            simpl;intros;try easy.   
-        }
-        {
-            intros.
-            simpl in H.
-            eapply IHn' in H.
-            f_equal;easy.
-        }   
-    }
-Qed.
-
-Lemma isMergeCtx_onth_inv : forall gss n  gs x, isMergeCtx gs gss -> 
-onth n gs= Some x -> exists k a, onth k gss=Some a /\
-onth n a = Some x.
-Proof.
-    induction gss.
-    {
-        intros.
-        inversion H.   
-    }
-    {
-        intros * Hmerge Honth.
-        inversion Hmerge;subst;
-        [exists 0, gs;crush |
-        
-        eapply IHgss in Honth;try easy;
-        destr_hyps;
-        exists (S x0), (x1);crush|].
-        eapply triple_sum_trilemma in H2;try exact Honth.
-        destruct H2.
-        {
-            eapply IHgss in H3;try exact H. destr_hyps.
-            exists (S x0), x1. crush.
-        }
-        {
-            exists 0. exists t';crush.
-        }
-    }
-Qed. 
-
-
-Lemma grafting_means_path : forall gx gs g g' n, 
-typ_gtth gs gx g ->
-usedCtx gs gx ->
-wfgC g ->
-onth n gs= Some g' ->
-    gttstepC_RT g g'.
-Proof.
-    induction gx using gtth_ind_ref.
-    {
-        intros * Hgraft Hused Hwfg Honth.
-        inversion Hgraft;inversion Hused;subst.
-        destruct (Nat.eq_dec n0 n);subst.
-         
-        try rewrite extendExtract in *. inversion Honth;inversion H1;subst.
-        eapply rt_refl.
-
-        eapply extend_onth_inv in Honth;subst;try easy.
-    }
-    {
-        
-        intros * Hgraft Hused Hwfg Honth.
-        
-        inversion Hused;subst.
-        inversion Hgraft;subst.
-        eapply isMergeCtx_onth_inv in H3 as Hmerge_onth;try exact Honth;destr_hyps.
-        rename x0 into gs'.
-        eapply Forall2_prop_r in H5;try exact H0.
-        tac_sanitize.
-        eapply Forall2_prop_r in H8;try exact H5;tac_sanitize.
-        rename x1 into gs', x4 into s, x5 into gh, x6 into gc.
-        eapply Forall_prop in H;try exact H5;tac_sanitize.
-        assert(Hstep: gttstepC (gtt_send p q ys) gc p q x).
-        {
-            pfold;econstructor.
-            apply wfgC_triv in Hwfg;try easy.
-            symmetry;exact H8.   
-        }
-        assert(Hrest: gttstepC_RT gc g').
-        {
-            eapply H2 with (gs:=gs') (n:=n);try easy.
-            eapply decidable_helper.typh_with_less;try exact H9;try easy.
-            eapply mergeCtx_onth_subset;try exact H3;try exact H0.
-            eapply continuation_wfgC;try exact H8;try exact Hwfg.
-        }
-        eapply rt_trans;try exact Hrest.
-        eapply rt_step;red;exists p, q, x;easy.
-    }
-Qed.   
-
-Lemma gttstep_preserves_wfg: forall g g', wfgC g -> projectableA g -> 
-gttstepC_RT g g' -> wfgC g' /\ projectableA g'.
-Proof.
-    intros.
-    induction H1. red in H1. destr_hyps.
-    split;[eapply wfgC_after_step| eapply projectable_after_step];try exact H1;try easy.
-    all:crush.
-Qed.
-Lemma wfg_list_by_grafting: forall gs gx g,typ_gtth gs gx g ->
-wfgC g -> projectableA g -> usedCtx gs gx ->
-forall_projable gs /\ forall_wfg gs.
-Proof. 
-    intros.
-    split;eapply Forall_forall;
-    intros;destruct x;crush;eapply in_some_implies_onth in H3;destr_hyps;
-    right;eapply grafting_means_path in H3;try exact H;try easy;exists g0;crush;
-    try apply gttstep_preserves_wfg in H3;try easy.
-Qed.
-
-Lemma gttstep_reflects_part : forall g g' r, wfgC g -> projectableA g -> isgPartsC r g' -> gttstepC_RT g g'->
-isgPartsC r g.
-Proof.
-    intros * Hwfg Hproj Hisparts Hstep.
-    induction Hstep;crush;
-    [red in H;destr_hyps;
-    eapply part_after_step_redux;try exact H|];crush.
-    eapply H0;eapply IHHstep2;try easy;eapply gttstep_preserves_wfg; try exact Hstep1;try easy.
-Qed.
-
-Lemma projectable_onth: forall xs p q k s a, wfgC (gtt_send p q xs) -> projectableA (gtt_send p q xs) ->
-onth k xs =Some (s,a) -> projectableA a.
-Proof.
-    intros.
-    eapply projectable_after_step with (g:=(gtt_send p q xs)) (p:=p) (q:=q) (ell:=k);try easy.
-    pfold. econstructor;[apply wfgC_triv in H;easy|symmetry;exact H1].
-Qed.
-
-Lemma Forall_onth_generic {A:Type}: forall (gcs1:list (option A)), 
-Forall (fun u=> u=None \/ exists k, onth k gcs1=u) gcs1.
-Proof.
-    induction gcs1;constructor.
-    destruct a; [right; exists  0 | left ];crush.
-    set (P:=(fun u  =>
-u = None \/ (exists k : opt_lbl, onth k gcs1 = u))).
-    eapply Forall_impl with (P:=P); unfold P in *;crush.
-    destruct (onth x gcs1) eqn:Hyg;[
-    eapply Forall_prop with (l:=x) (p:=a0) in IHgcs1|];crush.
-    right; exists (S x0); crush.
-Qed.
-
-
-Definition opt_list_subset {A:Type} (gs' gs :list (option A)) := 
-Forall2R  (fun u v : option A => u = None \/ u = v) gs' gs.
-
-Lemma projectionH_with_more_gs : forall gx gs' gs  p ls lx, 
-projectionH  gx gs' p lx ls -> opt_list_subset gs' gs -> projectionH gx gs p lx ls.
-Proof.
-    induction gx using gtth_ind_ref.
-    {
-        intros.
-        inversion H;subst.
-        red in H0;eapply Forall2R_prop in H0;try exact H2;destr_hyps.
-        destruct H1;try easy;subst.
-        
-        econstructor;try exact H4;crush.
-    }
-    {
-        intros. inversion H0;subst.
-        {
-            econstructor;try easy.
-            eapply Forall2_forall.
-            tac_forall_to_length;crush.
-            intros.
-            destruct (onth k xs) eqn:Hyg.
-            {
-                right.
-                eapply Forall_prop in H as IH;try exact Hyg;tac_sanitize.
-                
-                eapply Forall2_prop_r in H10 as Heqpr;try exact Hyg;tac_sanitize.
-                exists x2,x3,x4.
-                repeat split;try easy.
-                eapply H3;try easy H6;try exact H1;easy.
-            }   
-            {
-                destruct (onth k ys) eqn:Hyg'.
-                eapply Forall2_prop_l in H10 as Heqpr;try exact Hyg'; tac_sanitize;crush.
-                left. tauto.
-            }
-        }
-        {
-            econstructor;try easy.
-            eapply Forall2_forall.
-            tac_forall_to_length;crush.
-            intros.
-            destruct (onth k xs) eqn:Hyg.
-            {
-                right.
-                eapply Forall_prop in H as IH;try exact Hyg;tac_sanitize.
-                
-                eapply Forall2_prop_r in H10 as Heqpr;try exact Hyg;tac_sanitize.
-                exists x2,x3,x4.
-                repeat split;try easy.
-                eapply H3;try easy H6;try exact H1;easy.
-            }   
-            {
-                destruct (onth k ys) eqn:Hyg'.
-                eapply Forall2_prop_l in H10 as Heqpr;try exact Hyg'; tac_sanitize;crush.
-                left. tauto.
-            }
-        }
-        {
-            eapply projectionH_cont with (ys:=ys) (k:=k) (twt:=twt);try easy.
-            eapply Forall2_forall .
-            
-            tac_forall_to_length;crush.
-            rename k into ksl.
-            intros.
-            destruct (onth k xs) eqn:Hyg.
-            {
-                right.
-                eapply Forall_prop in H as IH;try exact Hyg;tac_sanitize.
-                
-                eapply Forall2_prop_r in H8 as Heqpr;try exact Hyg;tac_sanitize.
-                eapply Forall_prop in H14;try exact H9;tac_sanitize.
-                
-                exists x2,x3,x.
-                repeat split;try easy.
-                eapply H3;try easy H6;try exact H1;easy.
-            }   
-            {
-                destruct (onth k ys) eqn:Hyg'.
-                eapply Forall2_prop_l in H8 as Heqpr;try exact Hyg'; tac_sanitize;crush.
-                left. tauto.
-            }
-        }
-        
-    }
-Qed.
- 
-
-(*ls is a superset of projlist gs*)
-Definition is_proj_list_subset gs q ls := Forall2R (fun u v => u=None  \/ exists g t, u=Some g /\ v=Some t /\ projectionC g q t) gs ls.
- 
-Ltac subtac_wfgth_by_onth := match goal with 
-                            [ Hwfgth : wfgtth (gtth_send ?p ?q ?xs),
-                            Honthkxs : onth ?k ?xs = Some (_,?x)
-                            |- wfgtth ?x] => inversion Hwfgth;subst;
-                            match goal with [Hfa: Forall _ ?xs |- _] =>
-                            eapply Forall_prop in Hfa;try exact Honthkxs;tac_sanitize;easy end
-                            end.
-            
-            
-
-        Ltac subtac_projable_by_onth := match goal with 
-            [ Hprojable : projectableA (gtt_send ?p ?q ?xs),
-            Honthys : onth ?k ?xs = Some (?s, ?g1)
-            |- projectableA ?g1] => 
-            eapply projectable_onth;try exact Hprojable;try exact Honthys;easy end.                            
-        
-         Ltac subtac_typh_with_less := match goal with 
-                [Hgraft_g': typ_gtth ?gs ?gh ?g',
-                Hmergesubs : Forall2R (fun u v : option gtt => u = None \/ u = v) ?gs' ?gs,
-                Hused: usedCtx ?gs' ?gh
-                |- typ_gtth ?gs' ?gh ?g'] => eapply decidable_helper.typh_with_less;
-                try exact Hgraft_g';try easy end.
-
-        Ltac subtac_wfg_by_onth :=match goal with [Hwfg : wfgC (gtt_send ?p ?q ?xs),
-            Honthys : onth ?k ?xs = Some (?s, ?g1)
-            |- wfgC ?g1] => 
-            eapply continuation_wfgC;try exact Hwfg;try exact Honthys;easy end.
-
-        Ltac subtac_ishparts_by_onth := match goal with 
-        [ Honthkxs : onth ?k ?xs = Some (?s, ?gh),
-        Hishparts: ishParts ?p0 (gtth_send ?p ?q ?xs) -> False
-        |- ishParts ?p0 ?gh -> False] => 
-        intros;apply inequality_by_not_ishparts in Hishparts as Hpp; apply Hishparts;eapply ha_sendr;try exact Honthkxs;try easy
-        end.
-
-
-Lemma typ_gtth_means_slist_gs : forall gx gs g, 
-wfgtth gx ->
-typ_gtth gs gx g -> exists k a, onth k gs = Some a.
-Proof.
-    induction gx using gtth_ind_ref.
-    {
-        intros * Hwfg Htyp.
-    
-        inversion Htyp;subst;exists n, g;easy.
-    }
-    {
-        intros * Hwfg Htyp.
-    
-        inversion Hwfg;subst;eapply slist_implies_some in H2;destr_hyps.
-        inversion Htyp;subst. eapply Forall2_prop_r in H8;try exact H0;tac_sanitize. 
-        
-        eapply Forall_prop in H;try exact H5;try exact H0;tac_sanitize;
-        eapply H1;try subtac_wfgth_by_onth;try exact H5.
-    }
-Qed.
-Lemma local_graft_send : forall gx gs p q g ls,
-typ_gtth gs gx g -> wfgC g -> wfgtth gx ->
-projectableA g ->
-(ishParts p gx -> False) ->
-Forall (fun u=> u=None\/ exists ys, u=Some (gtt_send p q ys
-)) gs -> usedCtx gs gx -> 
-is_proj_list_subset gs q ls -> 
-exists lx , projectionH gx gs q lx ls.
-Proof.
-    induction gx using gtth_ind_ref.
-    {
-        intros * Htyp Hwfg Hwfgth Hprojable  Hishparts Hresgraft Hused Hprojlist.
-        specialize (Hprojable q) as Hprojq. destr_hyps. rename x into Tq.
-        exists (ltth_hol n).
-        
-        inversion Hused;subst.
-        eapply Forall_prop in Hresgraft;[| rewrite extendExtract;reflexivity].
-        tac_sanitize.
-        inversion Htyp;subst. rewrite extendExtract in H2;inversion H2;subst.
-        pinversion H;try apply proj_mon;subst;try easy.
-        {
-            exfalso;apply H0;apply decidable_helper.triv_pt_q;try easy.   
-        }
-        eapply Forall2R_prop in Hprojlist;try (rewrite extendExtract;reflexivity).
-        tac_sanitize.
-        econstructor;try exact H3;try exact H6.
-        rewrite extendExtract;easy.
-    }
-    {
-         
-        intros * Htyp Hwfg Hwfgth Hprojable  Hishparts Hresgraft Hused Hprojlist.
-        red in Hprojlist.
-        inversion Htyp;subst;rename H5 into Hslist_xs;rename H6 into Hgraft_fa2.
-        specialize (Hprojable q0) as Hprojq0. destr_hyps. rename x into Tq, H0 into Hprojq0.
-        pinversion Hprojq0;try apply proj_mon;subst.
-        {
-            exfalso;apply H0.   
-            assert(exists k u, onth k gs = Some u) by 
-            (eapply typ_gtth_means_slist_gs;try exact Htyp;try easy).
-            destr_hyps.
-            eapply Forall_prop in Hresgraft;try exact H1;
-            tac_sanitize.
-            
-            eapply gttstep_reflects_part with (g':=(gtt_send p0 q0 x1));try easy.
-            apply decidable_helper.triv_pt_q;try easy.
-            eapply wfg_list_by_grafting in Hused as Hforalls;try exact Hwfg;try easy.
-            destr_hyps. eapply Forall_prop in H3;try exact H1;tac_sanitize;easy.
-            eapply grafting_means_path;try exact H1;try exact Htyp;try easy.
-        }
-         1-2:   assert(create_lx: forall xs1
-        (Hsubset: Forall (fun u=> u=None \/ exists k, onth k xs=u) xs1),
-        exists lx,
-            Forall2
-(fun (u : option (sort * gtth)) (v : option (sort * ltth)) =>
-u = None /\ v = None \/
-(exists (s : sort) (g0 : gtth) (t : ltth),
-u = Some (s, g0) /\ v = Some (s, t) /\ projectionH g0 gs q0 t ls)) xs1 lx
-            ) by
-                (
-                induction xs1;[intros;exists [];constructor|];
-                    intros;
-                    inversion Hsubset;subst;rename H2 into Hdil_a, 
-                    H4 into Hsubset_ind;
-                    destruct a; [|
-                        specialize (IHxs1 Hsubset_ind);
-                        destr_hyps;
-                        exists (None::x);
-                        constructor;crush];
-                    
-                        destruct Hdil_a;try easy;destr_hyps;
-                        rename x into k,  H0 into Honthkxs;
-                        eapply Forall_prop in H;try exact Honthkxs;
-                        tac_sanitize;
-                        rename H0 into IH1;
-                        eapply Forall2_prop_r in Hgraft_fa2;try exact Honthkxs;tac_sanitize;
-                        rename H1 into Honthys, H2 into Hgraft_g', x2 into s, x4 into g';
-                        inversion Hused;subst;
-                        eapply Forall2_prop_l in H5;try exact Honthkxs;tac_sanitize;
-                        
-                        eapply mergeCtx_onth_subset with (gs:=gs) in H0 as Hmergesubs;try easy;
-                        assert(Hwfg2: wfgC g') by subtac_wfg_by_onth;
-                        eapply IH1 with (p :=p0) (q:=q0) (gs:=x0)  in Hwfg2 as IH;try easy;
-                        rename x0 into gs', x1 into s,x2 into gh;
-                        try solve [subtac_projable_by_onth | subtac_wfgth_by_onth | 
-                        subtac_typh_with_less | subtac_ishparts_by_onth | 
-                            eapply Forall_subset with (gs:= gs);crush |
-                            destr_hyps;
-                            specialize (IHxs1 Hsubset_ind) as IHxs';
-                            destr_hyps;
-                            exists (Some (s,x)::x0);
-                            constructor;try easy;
-                            right; exists s, gh,x;
-                            repeat split;try easy;
-                            eapply projectionH_with_more_gs with (gs':=gs');
-                            try exact H;try easy
-                        |
-                            red;
-                            eapply Forall2_Forall;[tac_forall_to_length | ];
-                            intros;
-                            destruct (onth k0 gs') eqn:Hyg1;[right |left;easy];
-                            eapply Forall2R_prop in Hmergesubs;try exact Hyg1;destr_hyps;
-                            destruct H5;try easy;subst;symmetry in H5;
-                            eapply Forall2R_prop in Hprojlist;try exact H5;tac_sanitize;
-                            exists x0, x1; crush   
-                        ]                    
-                );
-            specialize (create_lx xs (Forall_onth_generic xs)) as lx_gen;
-            destruct lx_gen as [lx lxprop].
-            exists (ltth_recv p lx); 
-                constructor;try easy.
-            exists (ltth_send q lx); 
-                constructor;try easy.
-
-        assert (create_lx: forall xs1
-        (Hsubset: Forall (fun u=> u=None \/ exists k, onth k xs=u) xs1),
-        exists lxs,
-            Forall2
-(fun (u : option (sort * gtth)) (v : option ltth) =>
-u = None /\ v = None \/
-(exists (s : sort) (g : gtth) (t0 : ltth),
-u = Some (s, g) /\ v = Some t0 /\ projectionH g gs q0 t0
-ls)) xs1 lxs /\
-        Forall
-        (fun u : option ltth =>
-        u = None \/ (exists th : ltth, u = Some th /\
-        typ_ltth th ls Tq)) lxs
-            ).
-            {
-                induction xs1;[intros;exists [];split;constructor|].
-                intros. inversion Hsubset;subst;rename H7 into Hsubsrest.
-                destruct a.
-                {
-                    destruct H2;try easy; destruct H0 as [k Honthkxs].
-                    eapply Forall2_prop_r in Hgraft_fa2;try exact Honthkxs;tac_sanitize.
-                    eapply Forall2_prop_r in H9;try exact H2;tac_sanitize.
-                    eapply Forall_prop in H;try exact Honthkxs;
-                    tac_sanitize.
-                    rename x0 into gh', x into s, x4 into g', x5 into twt.
-                    inversion Hused;subst.
-                    eapply Forall2_prop_l in H14;try exact Honthkxs;tac_sanitize.
-                    rename x2 into gh', x0 into gs',x1 into s.
-                    eapply mergeCtx_onth_subset in H1;try exact H12;try easy.
-                    Check mergeCtx_onth_subset.
-                    assert(Hwfg2: wfgC g') by subtac_wfg_by_onth.
-                    eapply H0 with (gs:=gs') (q:=q0) (ls:=ls) (p:=p0) in Hwfg2;try easy;
-                    try solve [subtac_ishparts_by_onth | subtac_projable_by_onth | subtac_wfgth_by_onth 
-                    | subtac_typh_with_less | 
-                        eapply Forall_subset in Hresgraft;try exact H1;try auto].
-                    {
-                        destruct Hwfg2 as [lxh Hlxh].
-                        specialize (IHxs1 Hsubsrest) as Hst;destruct Hst as [lxrest [Hrest1 Hrest2]].
-                        exists  (Some lxh::lxrest).
-                        split;constructor;try easy.
-                        right. exists s, gh', lxh;repeat split;try easy.
-                        eapply projectionH_with_more_gs;try exact Hlxh;red;easy.
-                        right. exists lxh;split;try easy.
-                        assert(Tq=twt) by (eapply merge_inv_ss in H10;try exact H8;easy);subst. 
-                        eapply projectionH_consistent with (g:=g') (p:=p0);try exact Hlxh;try easy;
-                        try solve [subtac_wfg_by_onth | subtac_wfgth_by_onth | destruct H9;easy].
-                        red;repeat split;try easy;try solve 
-                        [subtac_typh_with_less | subtac_ishparts_by_onth].
-                        eapply Forall_subset in Hresgraft;try exact H1;try auto.
-                        eapply Forall_impl;try exact Hresgraft;intros;simpl in H; destruct H;subst;
-                        try tauto;
-                        destr_hyps;subst;right;exists q0, x;tauto.
-                    }
-                    {
-                            red;
-                            eapply Forall2_Forall;[tac_forall_to_length | ];
-                            intros;
-                            destruct (onth k0 gs') eqn:Hyg1;[right |left;easy].
-                            eapply Forall2R_prop in H1;try exact Hyg1;destr_hyps.
-                            destruct H11;try easy;subst; symmetry in H11;
-                            eapply Forall2R_prop in Hprojlist;try exact H11;tac_sanitize;
-                            exists x0, x1; crush.   
-                    }
-                }
-                {
-                    specialize (IHxs1 Hsubsrest);
-                        destr_hyps;
-                        exists (None::x);
-                        constructor;crush.
-                }
-            }
-            specialize (create_lx xs (Forall_onth_generic xs)) as lx_gen.
-            destruct lx_gen as [lx [lx_prop1 lx_prop2]].
-            assert(Hxssome: SList xs) by (inversion Hwfgth;easy).
-            eapply slist_implies_some in Hxssome;destr_hyps.
-            eapply Forall2_prop_r in lx_prop1 as Hf2;try exact H0;
-            tac_sanitize.
-            exists x4. eapply projectionH_cont with (twt:=Tq);try exact H7;try easy.
-        
-    }
-Qed.
-
-Lemma typ_gtth_means_wfgtth : forall gx gs g, typ_gtth gs gx g -> wfgtth gx.
-Proof.
-    induction gx using gtth_ind_ref.
-    {
-        intros; constructor.
-    }
-    {
-        intros;constructor;[inversion H0;try easy |].
-        
-        eapply Forall_forall;intros;destruct x;try tauto; right;eapply in_some_implies_onth in H1;destr_hyps.
-        inversion H0;subst. eapply Forall2_prop_r in H8;try exact H1;tac_sanitize.
-        eapply Forall_prop in H;try exact H1;tac_sanitize; exists x0, x4;split;try easy;eapply H2;try exact H5.   
-    } 
-Qed.
-
-Lemma local_types_corr_send : forall p q xs Tq g, 
-wfgC g ->  projectionC g p (ltt_send q xs) ->
-projectableA g ->
-projectionC g q Tq -> exists ls ctx, typ_ltth ls ctx Tq.
-Proof.
-    intros * Hwfg Hprojp Hprojable Hprojq.
-    assert(Hisparts:isgPartsC p g). {
-        eapply projection_implies_part_send;try exact Hprojp.
-    }
-    eapply balanced_to_tree in Hisparts as Hgraft;try easy.
+    intros * Hwfg Hprojable Hproj.
+    assert(Hispartsp : isgPartsC p g ) by
+    (eapply projection_implies_part_send;try exact Hproj).
+    eapply balanced_to_tree in Hispartsp as Hss;try exact Hwfg;destr_hyps.
+    eapply restricted_grafting_send in H1;try exact H;try exact Hproj;try easy.
+    split. eapply projection_implies_part_send;try exact Hproj.
+    Search isgPartsC gttstepC_RT.
+    eapply   typ_gtth_means_slist_gs in H as ?Ht;try easy; try eapply typ_gtth_means_wfgtth;try exact H.
     destr_hyps.
-    assert (Htypp: typ_p_gtth x0 x p g) by (red;crush).
-    eapply typ_gtth_means_wfgtth in H as Hwfgth.
-    eapply wfg_list_by_grafting in H as Hlist_wfg;try easy.
-    eapply restricted_grafting_send with (ctx:=x) in H1;try exact Hprojp;try easy.
-    eapply project_list in H1 as Hprojs;try easy.
-    destruct Hprojs as [ls [?Hls ?Hls]].
-    eapply local_graft_send with (ls:=ls) (p:=p) (q:=q) in H as Hgetlx;try easy;destr_hyps.
-    eapply projectionH_consistent with (p:=p) in H3 as Hprojcons;try exact Hprojq;try easy.
-    exists x1, ls;easy.
-    
-    red;eapply Forall2_Forall;[tac_forall_to_length|];intros;
-    destruct (onth k x0) eqn:Hyg;try tauto;right.
-    eapply Forall2_prop_r in Hls;try exact Hyg;tac_sanitize;exists x2, x3;auto.
+    eapply gttstep_reflects_part with (g':=x2);try easy.
+    eapply Forall_prop in H1;try exact H3;destruct H1;try easy;destr_hyps;inversion H1;subst.
+    eapply wfg_list_by_grafting in H;try easy;destr_hyps.
+    red in H4. eapply Forall_prop in H4;try exact H3;tac_sanitize.
+    apply decidable_helper.triv_pt_q;easy.
+    eapply grafting_means_path;try exact H;try exact H3;easy.
 Qed.
 
-Lemma multigraft_proper_pref : forall p q g xs,
+
+Lemma proj_contains_q_implies_part_recv : forall g p q xs,
+wfgC g -> projectableA g ->
+projectionC g p (ltt_recv q xs) ->
+
+isgPartsC p g/\ isgPartsC q g.
+Proof.
+    intros * Hwfg Hprojable Hproj.
+    assert(Hispartsp : isgPartsC p g ) by
+    (eapply projection_implies_part_recv;try exact Hproj).
+    eapply balanced_to_tree in Hispartsp as Hss;try exact Hwfg;destr_hyps.
+    eapply restricted_grafting_recv in H1;try exact H;try exact Hproj;try easy.
+    split;try easy.
+    Search isgPartsC gttstepC_RT.
+    eapply   typ_gtth_means_slist_gs in H as ?Ht;try easy; try eapply typ_gtth_means_wfgtth;try exact H.
+    destr_hyps.
+    eapply gttstep_reflects_part with (g':=x2);try easy.
+    eapply Forall_prop in H1;try exact H3;destruct H1;try easy;destr_hyps;inversion H1;subst.
+    eapply wfg_list_by_grafting in H;try easy;destr_hyps.
+    red in H4. eapply Forall_prop in H4;try exact H3;tac_sanitize.
+    apply decidable_helper.triv_pt_p;easy.
+    eapply grafting_means_path;try exact H;try exact H3;easy.
+Qed.
+
+Lemma multigrafting_lemma_1 : forall  ctx_q p q g xs Tq gs_p gs_q ctx_p ,
 wfgC g -> projectableA g -> projectionC g p (ltt_send q xs) ->
-(forall ys, ~ projectionC g q (ltt_recv p ys)) ->
-exists gs_p ctx_p gs_q ctx_q,
-typ_p_gtth gs_p ctx_p p g /\ typ_p_gtth gs_q ctx_q q g /\
-is_tree_proper_prefix ctx_q ctx_p.
+projectionC g q Tq -> typ_p_gtth gs_p ctx_p p g -> 
+usedCtx gs_p ctx_p ->
+typ_p_gtth gs_q ctx_q q g ->
+usedCtx gs_q ctx_q -> gtth_eq ctx_p ctx_q -> exists ys, Tq =ltt_recv p ys.
 Proof.
-    intros * Hwfg Hprojable Hprojp Hnprojq.
-    assert(Hispartsp: isgPartsC p g) by admit.
-    assert(Hispartsq: isgPartsC q g) by admit.
-    eapply balanced_to_tree in Hispartsp as Hgraft;try easy.
-    destr_hyps.
-    rename x0 into gs_p, x into ctx_p.
-    eapply restricted_grafting_send with (ctx:=ctx_p) (q:=q)  (g:=g) (xs:=xs) in H1 as Hrg; try easy.
-    clear H1.
-    rename H into Hgraftp, H2 into Husedctxp, H0 into Hishpartsp.
-    eapply balanced_to_tree in Hispartsq as Hgraft;try easy.
-    destr_hyps.
-    rename x0 into gs_q, x into ctx_q, H into Hgraftq, H1 into Htri_q, H2 into Husedctxq, H0 into Hishpartsq. 
-    exists gs_p, ctx_p, gs_q, ctx_q.
-Admitted.
+    induction ctx_q using gtth_ind_ref.
+    {
+        intros * Hwfg Hprojable Hprojp Hprojq Htypp Husedp Htypq Husedq Hgttheq.
+        inversion Hgttheq;subst.
+        destruct Htypp as [?Htypp [?Htypp ?Htypp]].
+        destruct Htypq as [?Htypq [?Htypq ?Htypq]].
+        inversion Htypp;inversion Htypq;subst.
+        eapply restricted_grafting_send in Htypp;try exact Hprojp;try easy.
+        eapply Forall_prop in Htypp;try exact H1;tac_sanitize.
+        pinversion Hprojq;try apply proj_mon;subst;
+        [
+        exfalso;apply H;apply decidable_helper.triv_pt_q |
+        exists ys |
+        eapply wfgC_triv in Hwfg|
+        ];easy.
+    }
+    {
+        
+        intros * Hwfg Hprojable Hprojp Hprojq Htypp Husedp Htypq Husedq Hgttheq.
+        Search projectionC isgPartsC ltt_send.
+        assert (Hispartsp : isgPartsC p0 g) by (eapply proj_contains_q_implies_part_send in Hprojp;try easy).
+        assert (Hispartsq : isgPartsC q0 g) by (eapply proj_contains_q_implies_part_send in Hprojp;try easy).
+        
+        inversion Hgttheq;subst.
+        destruct Htypp as [?Htypp [?Htypp ?Htypp]].
+        destruct Htypq as [?Htypq [?Htypq ?Htypq]].
+        rename H2 into Hgtth_eqfa2, xs into xsq, xs1 into xsp.
+        
+        eapply restricted_grafting_send in Htypp as Hrg;try exact Hprojp;try easy.
+        pinversion Hprojq;try apply proj_mon;subst;try easy.
+        {
+            inversion Htypq;subst.
+            exfalso;apply Htypq0;apply ha_sendq.   
+        }
+        {
+            inversion Htypq;subst. 
+            exfalso;apply Htypq0;apply ha_sendp.     
+        }
+        {
+            inversion Htypq;subst.
+            eapply merge_slist in H5 as Hmergeslist.
+            eapply slist_implies_some in Hmergeslist;destr_hyps.
+            eapply Forall2_prop_l in H4;try exact H6;tac_sanitize.
+            eapply Forall2_prop_l in H14;try exact H7;tac_sanitize.
+            eapply Forall_prop in H;try exact H8;tac_sanitize.
+            eapply Forall2_prop_l in Hgtth_eqfa2;try exact H8;tac_sanitize.
+            eapply merge_inv_ss in H6;try exact H5;try easy;subst.
+            destruct H10;try easy.
+            inversion Husedq;subst.
+            inversion Husedp;subst.
+            eapply Forall2_prop_l in H17;try exact H8;tac_sanitize.
+            eapply Forall2_prop_l in H19;try exact H11;tac_sanitize.
+            rename x1 into gs_q', x3 into gs_p', x4 into ghq, x into k,
+            x8 into ghp, x7 into s, x6 into g'.
+            eapply mergeCtx_onth_subset in H10;try exact H15.
+            eapply mergeCtx_onth_subset in H13;try exact H16.
+            eapply H4 with (p:=p0) (xs:=xs0) (ctx_p:=ghp) (gs_p:=gs_p') (gs_q:=gs_q') in H;try easy.
+            subtac_wfg_by_onth. subtac_projable_by_onth.
+            {
+                pinversion Hprojp;subst;try apply proj_mon.   
+                exfalso;apply Htypq0;apply ha_sendq.
 
+                eapply Forall2_prop_r in H27;try exact H7;tac_sanitize.
+                destruct H25;try easy.
+                eapply merge_inv_ss in H28;try exact H20;subst;easy.
+            }
+            {
+                red;repeat split.   
+                inversion Htypp;subst.
+                eapply Forall2_prop_l in H24;try exact H7;tac_sanitize.
+                rewrite H18 in H11;inversion H11;subst;clear H11.
+                eapply decidable_helper.typh_with_less;try exact H22;try easy.
+                subtac_ishparts_by_onth.
+                eapply Forall_subset;try exact H10;try exact Htypp1;try easy;auto.
+            }
+            {
+                red;repeat split.   
+                inversion Htypq;subst.
+                eapply Forall2_prop_l in H24;try exact H7;tac_sanitize.
+                rewrite H18 in H8;inversion H8;subst;clear H8.
+                eapply decidable_helper.typh_with_less;try exact H22;try easy.
+                subtac_ishparts_by_onth.
+                eapply Forall_subset;try exact H13;try exact Htypq1;try easy;auto.
+            }
+        }
+    }
+Qed.
 
-Section assoc_live_path_helpers.
-Variables (gamma: tctx) (g: gtt).
-Hypotheses (Hwfg: wfgC g) (Hwfltt: tctx_wf gamma) (Hassoc: assoc gamma g).
-Variables (pth:Path).
-Hypotheses (Hvalid_pth: valid_pathC pth) (Hfair: fair_path pth) (Hpath_start: path_starts_with gamma pth).
-Check eventually.
+Ltac subtac_triv_isparts_false := match goal with 
+    [H: ishParts ?p (gtth_send ?p ?q ?xs) -> False|- _] => exfalso; apply H;apply ha_sendp
+    | [H: ishParts ?q (gtth_send ?p ?q ?xs) -> False|- _] => exfalso; apply H;apply ha_sendq
+    | [H: isgPartsC ?p (gtt_send ?p ?q ?xs) -> False|- _] => exfalso; apply H;apply decidable_helper.triv_pt_p;try easy
+    | [H: isgPartsC ?q (gtt_send ?p ?q ?xs) -> False|- _] => exfalso; apply H;apply decidable_helper.triv_pt_q;try easy
+    end.
 
-Check typ_p_gtth.
-
-
-
-End assoc_live_path_helpers.
-
-Check local_types_corr_send.
-
-Lemma multigrafting_lemma_send :
-forall gamma',
-tctxR gamma (lsend p q (Some s) ell) gamma' ->
-exists gsp gsq ctx_p ctx_q, typ_p_gtth gsp ctx_p p g /\
-typ_p_gtth gsq ctx_q q g /\ typ_p_ltth ls lctx q 
-
-
-
-Lemma assoc_live_path_send : forall p q xsp, M.find p gamma= Some (ltt_send q xsp) ->
-eventually (enabled (fun u=> exists xsq, M.find q u = Some (ltt_recv p xsq))) pth. 
+Lemma multigrafting_lemma_2 : forall  ctx_p p q g xs ys gs_p gs_q ctx_q ,
+wfgC g -> projectableA g -> projectionC g p (ltt_send q xs) ->
+projectionC g q (ltt_recv p ys) -> typ_p_gtth gs_p ctx_p p g -> 
+usedCtx gs_p ctx_p ->
+typ_p_gtth gs_q ctx_q q g ->
+usedCtx gs_q ctx_q -> gtth_eq ctx_p ctx_q.
 Proof.
-    intros * Hfindp.
-    Search assoc M.find.
-    constructor.
-Admitted.
+    induction ctx_p using gtth_ind_ref.
+    {
+        intros * Hwfg Hprojable Hprojp Hprojq Htypp Husedp Htypq Husedq.
+        destruct Htypp as [?Htypp [?Htypp ?Htypp]].
+        destruct Htypq as [?Htypq [?Htypq ?Htypq]].
+        inversion Htypp;subst.
+        inversion Htypq;subst.
+        constructor.
+        {   
+            eapply restricted_grafting_send in Htypp as Hrg;try exact Hprojp;try easy.
+            eapply Forall_prop in Hrg;try exact H1;tac_sanitize.
+            exfalso;apply Htypq0;apply ha_sendq.   
+        }
+    }
+    {
+        intros * Hwfg Hprojable Hprojp Hprojq Htypp Husedp Htypq Husedq.
+        destruct Htypp as [?Htypp [?Htypp ?Htypp]].
+        destruct Htypq as [?Htypq [?Htypq ?Htypq]].
+        inversion Htypp;subst.
+        inversion Htypq;subst.
+        eapply Forall_prop in Htypq1;try exact H0;destruct Htypq1;try easy;destr_hyps.
+        destruct H1;[|destruct H1].
+        {
+            inversion H1;subst.
+            pinversion Hprojq;try apply proj_mon;subst;try easy.   
+        }
+        {
+            inversion H1;subst.
+            pinversion Hprojq;try apply proj_mon;subst;try easy; subtac_triv_isparts_false.           
+        }
+        {
+         inversion H1.   
+        }
+        {
+            constructor.
+            eapply Forall2_forall;[tac_forall_to_length|].
+            intros;destruct (onth k xs) eqn:Hyg.
+            right. 
+            eapply Forall_prop in H;try exact Hyg;tac_sanitize.
+            eapply Forall2_prop_r in H6;try exact Hyg; tac_sanitize.
+            eapply Forall2_prop_l in H8;try exact H2;tac_sanitize.
+            exists x0, x3, x1;repeat split;try easy.
+            inversion Husedp;subst.
+            inversion Husedq;subst.
+            eapply Forall2_prop_l in H13;try exact H1;tac_sanitize.
+            eapply Forall2_prop_l in H11;try exact Hyg;tac_sanitize.
+            pinversion Hprojp;try apply proj_mon;subst;try subtac_triv_isparts_false.
+            pinversion Hprojq;try apply proj_mon;subst;try subtac_triv_isparts_false.
+            eapply Forall2_prop_r in H27;try exact H2;tac_sanitize.
+            eapply Forall2_prop_r in H21;try exact H2;tac_sanitize.
+            destruct H25;destruct H26;try easy.
+            eapply merge_inv_ss in H14;try exact H28;subst.
+            eapply merge_inv_ss in H21;try exact H22;subst.
+            eapply H0 with (gs_p:=x0) (gs_q:=x2) (g:=x5);try exact H;try exact H11;try easy.
+            subtac_wfg_by_onth. subtac_projable_by_onth.
+            {
+                red;repeat split;
+                eapply mergeCtx_onth_subset in H8;try exact H9.
+                eapply decidable_helper.typh_with_less;try exact H8;try easy.
+                subtac_ishparts_by_onth.
+                eapply Forall_subset;try exact H8;auto.
+            }
+            {
+                red;repeat split;
+                eapply mergeCtx_onth_subset in H6;try exact H10.
+                eapply decidable_helper.typh_with_less;try exact H7; try easy.
+                subtac_ishparts_by_onth.
+                eapply Forall_subset;try exact H6;auto.
+            }
+            left. split;try easy.
+            destruct (onth k xs1) eqn:Hyg2;try easy.
+            eapply Forall2_prop_r in H8;try exact Hyg2;tac_sanitize.
+            eapply Forall2_prop_l in H6;try exact H2;tac_sanitize.
+            rewrite Hyg in H1;try easy.
+        }
+    }
+Qed.
 
-End assoc_live_path_helpers.
+
+Ltac subtac_onth_typ Honthctxlist Hmerge:=
+red;repeat split;
+eapply mergeCtx_onth_subset in Honthctxlist as Hsubset;try exact Hmerge;
+[
+
+eapply decidable_helper.typh_with_less;try exact Hsubset;try easy
+|
+    subtac_ishparts_by_onth|
+eapply Forall_subset;try exact Hsubset;auto].
+
+Ltac subtac_onth_solver := try solve [subtac_ishparts_by_onth  | subtac_projable_by_onth | subtac_triv_isparts_false | subtac_wfg_by_onth | subtac_wfgth_by_onth].
+
+Lemma multigrafting_lemma_3_send : forall  ctx_p p r q g xs ys gs_p gs_q ctx_q ,
+wfgC g -> projectableA g -> projectionC g p (ltt_send q xs) ->
+(projectionC g q (ltt_send r ys) \/ projectionC g q (ltt_recv r ys) ) -> r <> p -> typ_p_gtth gs_p ctx_p p g -> 
+usedCtx gs_p ctx_p ->
+typ_p_gtth gs_q ctx_q q g ->
+usedCtx gs_q ctx_q -> is_tree_proper_prefix ctx_q ctx_p.
+Proof.
+    induction ctx_p using gtth_ind_ref.
+    {
+        intros * Hwfg Hprojable Hprojp Hprojq Hrnp Htypp Husedp Htypq Husedq.
+        destruct Htypp as [?Htypp [?Htypp ?Htypp]].
+        destruct Htypq as [?Htypq [?Htypq ?Htypq]].
+        inversion Htypp;subst.
+        inversion Htypq;subst.
+        {
+            eapply restricted_grafting_send in Hprojp;try exact Htypp;try easy.
+            eapply Forall_prop in Hprojp;try exact H1.
+            destruct Hprojp;try easy;destr_hyps; inversion H0;subst;clear H0.                
+            destruct Hprojq as [Hprojq | Hprojq];
+            [eapply restricted_grafting_send in Hprojq|
+            eapply restricted_grafting_recv in Hprojq];
+            try exact Htypq;try easy;
+                eapply Forall_prop in Hprojq;try exact H;
+                destruct Hprojq;try easy;destr_hyps;inversion H0;subst;clear H0;easy.
+        }
+        {
+            eapply restricted_grafting_send in Hprojp;try exact Htypp;try easy.
+            eapply Forall_prop in Hprojp;try exact H1.
+            destruct Hprojp;try easy;destr_hyps; inversion H2;subst;clear H2.
+            subtac_triv_isparts_false.                
+        }
+    }
+    {
+        intros * Hwfg Hprojable Hprojp Hprojq Hrnp Htypp Husedp Htypq Husedq.
+        destruct Htypp as [?Htypp [?Htypp ?Htypp]].
+        destruct Htypq as [?Htypq [?Htypq ?Htypq]].
+        inversion Htypp;inversion Htypq;subst;[constructor |].
+        inversion H11;subst;clear H11.
+        constructor.
+        eapply Forall2_forall.
+        tac_forall_to_length.
+        intros.
+        destruct (onth k xs) eqn:Hyg.
+        {
+            right.
+            eapply Forall2_prop_r in H6;try exact Hyg;tac_sanitize.   
+            eapply Forall2_prop_l in H8;try exact H2;tac_sanitize.
+            exists x3, x4, x1.
+            repeat split;try easy.
+            inversion Husedp;subst.
+            inversion Husedq;subst.
+            eapply Forall2_prop_l in H13;try exact H1;tac_sanitize.
+
+            eapply Forall2_prop_l in H11;try exact Hyg;tac_sanitize.
+            
+            rename xs2 into ghsq,xs into ghsp, ys0 into gcs, x4 into s, x5 into g',
+            x7 into ghp, x6 into ghq, x0 into gs_q', x3 into gs_p'.
+            rename Hyg into Honthghsp, H2 into Honthgcs, H1 into Honthghsq.
+            eapply Forall_prop in H as IH;try exact Honthghsp;tac_sanitize.
+            rename x into s, x0 into ghp.
+            eapply H1 with (g:=g') (gs_p:=gs_p') (gs_q:=gs_q') (p:=p0) (q:=q0)
+            (xs:=xs0) (ys:=ys) (r:=r);try easy;
+            try solve [subtac_onth_solver | subtac_onth_typ H9 H8 | subtac_onth_typ H4 H10]. 
+            {
+                pinversion Hprojp;try apply proj_mon;subst.  subtac_triv_isparts_false.
+                eapply Forall2_prop_r in H20;try exact Honthgcs;tac_sanitize.
+                destruct H18;try easy.
+                eapply merge_inv_ss in H11;try exact H21;subst;easy. 
+            }
+            {
+                destruct Hprojq as [Hprojq | Hprojq];
+                 pinversion Hprojq;try apply proj_mon;subst;  try subtac_triv_isparts_false;
+                eapply Forall2_prop_r in H20;try exact Honthgcs;tac_sanitize;
+                destruct H18;try easy;
+                eapply merge_inv_ss in H11;try exact H21;subst;auto.
+                
+            }
+        }
+        {
+            left. destruct (onth k xs2) eqn:Hyg2;try auto.
+            eapply Forall2_prop_r in H8;try exact Hyg2;tac_sanitize.
+            eapply Forall2_prop_l in H6;try exact H2;tac_sanitize.
+            rewrite H1 in Hyg;inversion Hyg;subst;easy.   
+        }
+    }
+Qed.    
+
+Lemma two_send_proj_impossible: forall   p q g xs ys ,
+wfgC g -> projectableA g -> projectionC g p (ltt_send q xs) ->
+projectionC g q (ltt_send p ys) -> False.
+Proof.
+Admitted.
+Lemma multigrafting_lemma : forall  ctx_q p q g xs Tq gs_p gs_q ctx_p ,
+wfgC g -> projectableA g -> projectionC g p (ltt_send q xs) ->
+projectionC g q Tq -> typ_p_gtth gs_p ctx_p p g -> 
+usedCtx gs_p ctx_p ->
+typ_p_gtth gs_q ctx_q q g ->
+usedCtx gs_q ctx_q ->
+(is_tree_proper_prefix ctx_q ctx_p) \/ (gtth_eq ctx_p ctx_q).
+Proof.
+    intros. destruct Tq.
+    {
+        Search projectionC ltt_end isgPartsC. 
+        eapply proj_contains_q_implies_part_send in H1;try easy;eapply pmergeCR in H2;
+        try easy.
+    }
+    {
+        destruct (Nat.eq_dec n p);subst.
+        right.
+        eapply multigrafting_lemma_2 with (gs_p:=gs_p) (gs_q:=gs_q) (p:=p) (q:=q); try exact H1;try exact H2;try easy.
+        
+        left.
+        eapply multigrafting_lemma_3_send with (gs_p:=gs_p) (gs_q:=gs_q) (r:=n) (p:=p) (q:=q) (ys:=l);try exact H1;try easy.
+        auto.
+    }
+    {
+        destruct (Nat.eq_dec n p);subst.
+        exfalso; eapply two_send_proj_impossible;try exact H1;try exact H2;try easy.
+        
+        left.
+        eapply multigrafting_lemma_3_send with (gs_p:=gs_p) (gs_q:=gs_q) (r:=n) (p:=p) (q:=q) (ys:=l);try exact H1;try easy.
+        auto.
+    }
+Qed.
+
+Lemma eventually_if : 
+forall (P Q : Path -> Prop) (xs:Path), eventually P xs -> 
+(forall ys, P ys -> eventually Q ys) -> eventually Q xs.
+Proof.
+    intros.
+    induction H;[crush|].
+
+    constructor 2. easy.
+Qed.
+
+Check Path.
+Definition head_contains_q_recv p q:=(
+    fun (pt:Path) => match pt with 
+        | cocons (hd,l) tl => exists ys, M.find q hd=Some (ltt_recv p ys)  
+        | _ => False end
+        ).
+Lemma assoc_live_helper_send : 
+forall gamma p q g  l pt_tl xs, fair_path (cocons (gamma,l) pt_tl) -> 
+valid_pathC (cocons (gamma,l) pt_tl) -> tctx_wf gamma -> wfgC g ->
+assoc gamma g -> 
+M.find p gamma= Some (ltt_send q xs) -> eventually (
+    head_contains_q_recv p q
+        ) (cocons (gamma,l) pt_tl) .
+Proof.
+    intros * Hfair Hvalid Htctxwf Hwfg Hassoc Hfindp.
+    assert(Hprojable:projectableA g) by 
+    (eapply assoc_implies_projectable;try exact Hassoc;easy).
+    assert (Hispartsp : isgPartsC p g) by
+    (eapply assoc_implies_part;try exact Hfindp;try easy).
+    Print tac_use_assoc.   
+    tac_use_assoc Hassoc p Hispartsp;destr_hyps.
+    rewrite Hfindp in H;inversion H;subst;clear H.
+    red in H0;destr_hyps. rename x into spty.
+    eapply subtype_send_inv1 in H0;destr_hyps;subst.
+    rename x into xsp.
+    eapply proj_contains_q_implies_part_send in H as Hispartsq;try easy.
+    destruct Hispartsq as [_  Hispartsq].
+    eapply balanced_to_tree in Hispartsp as Hgraftp;try easy.
+    destruct Hgraftp as [ctx_p [gs_p [?Hgraftp [?Hgraftp [?Hgraftp ?Hgraftp ]]]]].
+    eapply typ_gtth_means_wfgtth in Hgraftp as Hwfgth.
+    generalize dependent gs_p.
+    generalize dependent g.
+    generalize dependent gamma.
+    generalize dependent  pt_tl.
+    generalize dependent l.
+    revert Hgraftp0 xs xsp.
+    generalize dependent p.
+    generalize dependent q.
+    revert Hwfgth.
+    revert ctx_p.
+    induction ctx_p using gtth_ind_by_height.
+    {
+        intros. rename H into IH, H0 into Hprojp.
+        specialize (Hprojable q) as Ht.
+        destruct Ht as [Tq Hprojq].
+        eapply balanced_to_tree in Hispartsq as Hgraftq;try easy.
+        destruct Hgraftq as [ctx_q [gs_q [?Hgraftq [?Hgraftq [?Hgraftq ?Hgraftq]]]]].
+        eapply multigrafting_lemma with (q:=q) (p:=p) (gs_p:=gs_p) (ctx_p:=ctx_p)
+        (gs_q:=gs_q) (ctx_q:=ctx_q) (Tq:=Tq) in Hprojp as Hmg;try easy.
+        destruct Hmg.
+        {
+            admit.   
+        }
+        {
+            eapply multigrafting_lemma_1 with (g:=g) (p:=p) (q:=q) (gs_p:=gs_p)
+            (gs_q:=gs_q) (Tq:=Tq) (xs:=xsp)
+            in H;try easy.
+            destruct H as [ys H];subst.
+            tac_use_assoc Hassoc q Hispartsq.
+            destr_hyps. red in H0. destr_hyps. eapply proj_inj in H0;try exact Hprojq;subst;try easy.
+            eapply subtype_recv_inv2 in H1;destr_hyps;subst.
+            econstructor. red;simpl. exists x0;easy.
+        }
+    }
+    
+
+
 Lemma assoc_live_path:  forall gamma g, tctx_wf gamma -> wfgC g ->
 assoc gamma g -> liveCtx gamma.
 Proof.
@@ -1763,9 +520,9 @@ Proof.
     split.
     {
         intros.
-        simpl in H5. inversion H5.
-        Search "lem" "inv".   
+        simpl in H5. inversion H5.   
         eapply lem_6_11a_tctx_send_invert in H6. destr_hyps.
+        
         eapply assoc_live_path_send with (g:=g)  (pth:=(cocons (g', l) xs)) in H6;try easy.
         4:red.
     }
